Small cleanups and similar code move.

coquand_geometrical_logic/deduction.v
@@ -1,10 +1,44 @@
 Require List Eqdep_dec Lia.
 Require Import seq syntax.
 
+(* Nothing to do here, move me *)
+
 Lemma nat_uip : forall (m n : nat) (p q : m = n), p = q.
 Proof.
 intros; apply Eqdep_dec.UIP_dec.
 decide equality.
+Qed.
+
+Inductive In {A} (x : A) : list A -> Type :=
+| In_here : forall l, In x (cons x l)
+| In_next : forall y l, In x l -> In x (cons y l).
+
+Lemma In_app_l : forall (A : Type) (l1 l2 : list A) (x : A),
+  In x l1 -> In x (app l1 l2).
+Proof.
+intros A l1 l2 x H; revert l2; induction H; intros l2; simpl; constructor; intuition.
+Qed.
+
+Lemma In_app_r : forall (A : Type) (l1 l2 : list A) (x : A),
+  In x l2 -> In x (app l1 l2).
+Proof.
+induction l1; intros l2 x H; cbn in *; [assumption|].
+constructor; apply IHl1, H.
+Qed.
+
+Lemma In_map : forall (A B : Type) (f : A -> B) (l : list A) (x : A),
+  In x l -> In (f x) (List.map f l).
+Proof.
+induction 1; constructor; assumption.
+Qed.
+
+Lemma In_map_rev : forall (A B : Type) (f : A -> B) (l : list A) (y : B),
+  In y (List.map f l) -> {x : A & prod (In x l) (y = f x)}.
+Proof.
+intros A B f l y H; induction l as [|x l IHl]; cbn in *; inversion H; subst.
++ repeat econstructor.
++ destruct IHl as [x' [? ?]]; [assumption|].
+  exists x'; repeat constructor; assumption.
 Qed.
 
 Set Primitive Projections.
@@ -15,13 +49,9 @@ Context {Sig : sig}.
 Notation form := (@form Sig).
 
 Record Theory := {
-  thy_idx : Set;
+  thy_idx : Type;
   thy_axm : forall i : thy_idx, form 0;
 }.
-
-Inductive In {A} (x : A) : list A -> Type :=
-| In_here : forall l, In x (cons x l) 
-| In_next : forall y l, In x l -> In x (cons y l).
 
 Definition lift_form {Σ : nat} (A : form Σ) : form (S Σ) :=
   subst_form (init (fun n => @var_term _ (S _) (Some n))) A.
@@ -46,11 +76,11 @@ Inductive proof (T : Theory) (Σ : nat) (Γ : list (form Σ)) : form Σ -> Type 
   proof T Σ Γ (Cnj A B) -> proof T Σ Γ A
 | prf_cnj_e₂ : forall A B,
   proof T Σ Γ (Cnj A B) -> proof T Σ Γ B
-| prj_dsj_i₁ : forall A B,
+| prf_dsj_i₁ : forall A B,
   proof T Σ Γ A -> proof T Σ Γ (Dsj A B)
-| prj_dsj_i₂ : forall A B,
+| prf_dsj_i₂ : forall A B,
   proof T Σ Γ B -> proof T Σ Γ (Dsj A B)
-| prj_dsj_e : forall A B C,
+| prf_dsj_e : forall A B C,
   proof T Σ Γ (Dsj A B) -> proof T Σ (cons A Γ) C -> proof T Σ (cons B Γ) C -> proof T Σ Γ C
 | prf_frl_i :
   forall (A : form (S Σ)), proof T (S Σ) (List.map lift_form Γ) A -> proof T Σ Γ (All A) 
@@ -67,12 +97,66 @@ Inductive proof (T : Theory) (Σ : nat) (Γ : list (form Σ)) : form Σ -> Type 
   proof T Σ Γ B
 .
 
-Lemma map_init_eta : forall Σ Σ' t (ρ : seq (@term Sig Σ) Σ'),
-  init (funcomp var_term shift) >> scons t ρ = ρ.
+(* Derived rules *)
+
+Lemma prf_wkn : forall T Σ Γ Δ A, (forall X, In X Γ -> In X Δ) -> proof T Σ Γ A -> proof T Σ Δ A.
 Proof.
-intros.
-rewrite map_init; apply nth_ext; intros n.
-rewrite nth_init; reflexivity.
+intros T Σ Γ Δ A Hi H; revert Δ Hi; induction H; intros Δ Hi; try (solve [econstructor; eauto]).
++ apply prf_arr_i, IHproof.
+  { intros X HX; inversion HX; subst; constructor; now intuition. }
++ eapply prf_dsj_e; [apply IHproof1, Hi|apply IHproof2|apply IHproof3].
+  all: intros X HX; inversion HX; subst; constructor; now intuition.
++ apply prf_frl_i, IHproof.
+  { intros X HX. apply In_map_rev in HX; destruct HX as [Y [HY ->]].
+    apply In_map, Hi, HY. }
++ eapply prf_exs_e; [apply IHproof1, Hi|apply IHproof2].
+  { intros X HX. apply In_map_rev in HX; destruct HX as [Y [HY ->]].
+    apply In_map, Hi, HY. }
+Qed.
+
+Lemma prf_subst : forall T Σ Σ' Γ A (ρ : seq (term Σ') Σ),
+  proof T Σ Γ A -> proof T Σ' (List.map (subst_form ρ) Γ) (subst_form ρ A).
+Proof.
+intros T Σ Σ' Γ A ρ p; revert Σ' ρ; induction p; intros Σ' ρ; try (solve [econstructor; eauto]).
++ rewrite compComp_form.
+  apply prf_thy.
++ apply prf_axm, In_map; assumption.
++ cbn; apply prf_frl_i.
+  specialize (IHp (S Σ') (up_term_term ρ)).
+  match goal with [ _ : proof _ _ ?Γ _ |- proof _ _ ?Δ _ ] => replace Δ with Γ; [assumption|] end.
+  rewrite !List.map_map; apply List.map_ext; clear; intros A.
+  unfold lift_form; rewrite !compComp_form.
+  f_equal; apply nth_ext; intros n.
+  rewrite !nth_map, !nth_init; cbn.
+  rewrite !nth_map; reflexivity.
++ cbn in *.
+  rewrite compComp_form; simpl.
+  specialize (IHp Σ' ρ).
+  eapply prf_frl_e with (t := subst_term ρ t) in IHp.
+  match goal with [ _ : proof _ _ _ ?A |- proof _ _ _ ?B ] => replace B with A; [assumption|] end.
+  rewrite compComp_form; f_equal; simpl; f_equal.
+  apply nth_ext; clear; intros n; rewrite !nth_map, !compComp_term, !nth_init; simpl.
+  apply idSubst_term; clear; intros m; rewrite !nth_map, !nth_init; simpl; rewrite nth_init; reflexivity.
++ cbn in *; eapply prf_exs_i with (t := subst_term ρ t).
+  specialize (IHp Σ' ρ).
+  match goal with [ _ : proof _ _ _ ?A |- proof _ _ _ ?B ] => replace B with A; [assumption|] end.
+  rewrite !compComp_form; f_equal; apply nth_ext; clear; intros [n|]; [|reflexivity].
+  simpl; rewrite !nth_map, !compComp_term, !map_init; simpl.
+  rewrite idSubst_term.
+  2:{ clear; intros n; rewrite !nth_init; reflexivity. }
+  rewrite nth_init; reflexivity.
++ cbn in *. specialize (IHp1 Σ' ρ).
+  eapply prf_exs_e in IHp1; [now apply IHp1|].
+  specialize (IHp2 (S Σ') (up_term_term ρ)).
+  assert (e : forall A, subst_form (up_term_term ρ) (lift_form A) = lift_form (subst_form ρ A)).
+  { clear; intros A; unfold up_term_term, lift_form.
+    rewrite !compComp_form; f_equal; apply nth_ext; intros n.
+    rewrite !nth_map, !nth_init; simpl; rewrite !nth_map; reflexivity. }
+  match goal with [ _ : proof _ _ ?Γ ?A |- proof _ _ ?Δ ?B ] =>
+    replace Δ with Γ; [replace B with A|]; [assumption| |]
+  end.
+  - rewrite e; reflexivity.
+  - rewrite !List.map_map; apply List.map_ext; intros ?; apply e.
 Qed.
 
 End syntax.
